Pom.lean
@@ -1,2 +1,2 @@
 import Pom.Basic
-import Pom.Linearization
+import Pom.Semantics
